
### 常规
$$
\begin{align}
(a+b)^{2}= & a^{2}+2ab+b^{2} \\
(a-b)^{2}= & a^{2}-2ab+b^{2} \\
(a+b)^{3}= & a^{3}+3a^{2}b+3ab^{2}+b^{3} \\
(a-b)^{3}= & a^{3}-3a^{2}b+3ab^{2}-b^{3} \\
a^{2}-b^{2}= & (a+b)(a-b) \\
a^{3}-b^{3}= & (a-b)(a^{2}+ab+b^{2}) \\
a^{3}+b^{3}= & (a+b)(a^{2}-ab+b^{2}) \\
a^{n}-b^{n}= & (a-b)(a^{n-1}+a^{n-2}b+\cdots+ab^{n-2}+b^{n-1})~~(n是整数) \\
a^{n}+b^{n}= & (a+b)(a^{n-1}-a^{n-2}b+\cdots-ab^{n-2}+b^{n-1})~~(n是正齐数)\\
(a+b)^{n}= & \sum_{k=0}^{n} C_{n}^{k}a^{n-k}b^{k}~~(二项式定理)
\end{align}
$$

### 其他
$$
\begin{align} \\
来自题目  &  f\left( x+\frac{1}{x} \right)=\frac{{x+x^{3}}}{1+x^{4}},则f(x)=?\\
\frac{{x+x^{3}}}{1+x^{4}} = &  \frac{{\frac{1}{x}+x}}{\frac{1}{x^{2}}+x^{2}}~~(除以 二次方) \\
= & \frac{{\frac{1}{x}+x}}{\left( \frac{1}{x}+x \right)^{2}-2}~~(转换分母形式) \\
可知 f(x)= & \frac{x}{x^{2}-2}
\end{align}
$$

---
来自某个题目的 部分解题 过程
$$
\frac{1}{4n^{2}-1}=\frac{1}{(2n-1)(2n+1)}=\frac{1}{2}\left( \frac{1}{2n-1}-\frac{1}{2n+1} \right)
$$
$$
\frac{1}{a^{2}-b^{2}}= \frac{1}{(a-b)(a+b)}=\frac{1}{2b}\left( \frac{1}{a-b}-\frac{1}{a+b} \right)
$$
